ironfleet/src/Dafny/Distributed/Impl/SHT/PacketParsing.i.dfy
@@ -31,7 +31,7 @@ function method OptionalValue_grammar() : G { GTaggedUnion([Value_grammar(), GTu
 function method KeyPlus_grammar() : G { GTaggedUnion([Key_grammar(), GUint64]) }
 function method KeyRange_grammar() : G { GTuple([KeyPlus_grammar(), KeyPlus_grammar()]) }
 function method Hashtable_grammar() : G { GArray(GTuple([Key_grammar(), Value_grammar()])) }
-function method EndPoint_grammar() : G { GUint64 }
+function method EndPoint_grammar() : G { GByteArray }
 
 ////////////////////////////////////////////////////////////////////
 //    Grammars for the SHT messages 
@@ -141,10 +141,7 @@ function method parse_EndPoint(val:V) : EndPoint
     requires ValInGrammar(val, EndPoint_grammar());
     ensures  EndPointIsAbstractable(parse_EndPoint(val));
 {
-    if val.u <= 0xffffffffffff then
-        ConvertUint64ToEndPoint(val.u)
-    else
-        EndPoint([0,0,0,0], 0)
+    EndPoint(val.b)
 }
 
 function method parse_Message_GetRequest(val:V) : CMessage
@@ -285,14 +282,14 @@ predicate MessageMarshallable(msg:CMessage)
         case CGetRequest(k) => ValidKey(k)
         case CSetRequest(k, v) => ValidKey(k) && ValidOptionalValue(v) 
         case CReply(k, v) => ValidKey(k) && ValidOptionalValue(v) 
-        case CRedirect(k, id) => ValidKey(k) && EndPointIsAbstractable(id)
-        case CShard(kr, id) => ValidKeyRange(kr) && EndPointIsAbstractable(id) && !EmptyKeyRange(msg.kr)
+        case CRedirect(k, id) => ValidKey(k) && EndPointIsValidPublicKey(id)
+        case CShard(kr, id) => ValidKeyRange(kr) && EndPointIsValidPublicKey(id) && !EmptyKeyRange(msg.kr)
         case CDelegate(kr, h) => ValidKeyRange(kr) && ValidHashtable(h) && !EmptyKeyRange(msg.range)
 }
 
 predicate CSingleMessageMarshallable(msg:CSingleMessage) 
 {
-    msg.CAck? || (msg.CSingleMessage? && EndPointIsAbstractable(msg.dst) && MessageMarshallable(msg.m))
+    msg.CAck? || (msg.CSingleMessage? && EndPointIsValidPublicKey(msg.dst) && MessageMarshallable(msg.m))
 }
 
 method IsValidKeyPlus(kp:KeyPlus) returns (b:bool)
@@ -382,10 +379,10 @@ method IsMessageMarshallable(msg:CMessage) returns (b:bool)
             }
         case CRedirect(k, id) => 
             b := IsKeyValid(k);
-            b := b && (|id.addr| as uint64 == 4 && 0 <= id.port <= 65535);
+            b := b && (|id.public_key| < 0x10_0000);
         case CShard(kr, id) => 
             b := IsValidKeyRange(kr);
-            b := b && (|id.addr| as uint64 == 4 && 0 <= id.port <= 65535);
+            b := b && (|id.public_key| < 0x10_0000);
             if b {
                 b := IsEmptyKeyRange(kr);
                 b := !b;
@@ -413,7 +410,7 @@ method IsCSingleMessageMarshallable(msg:CSingleMessage) returns (b:bool)
     } else {
         assert msg.CSingleMessage?;
 
-        if !(|msg.dst.addr| as uint64 == 4 && 0 <= msg.dst.port <= 65535) {
+        if !(|msg.dst.public_key| < 0x10_0000) {
             b := false;
             return;
         }
@@ -580,13 +577,13 @@ method MarshallHashtable(c:Hashtable) returns (val:V)
 }
 
 method MarshallEndPoint(c:EndPoint) returns (val:V)
-    requires EndPointIsAbstractable(c);
-    ensures  ValInGrammar(val, EndPoint_grammar());
-    ensures  ValidVal(val);
-    ensures  parse_EndPoint(val) == c;
+    requires EndPointIsValidPublicKey(c)
+    ensures  ValInGrammar(val, EndPoint_grammar())
+    ensures  ValidVal(val)
+    ensures  parse_EndPoint(val) == c
+    ensures  0 <= SizeOfV(val) < 0x10_0008
 {
-    val := VUint64(ConvertEndPointToUint64(c));
-    Uint64EndPointRelationships();
+    val := VByteArray(c.public_key);
 }
 
 method MarshallMessage_GetRequest(c:CMessage) returns (val:V)
@@ -595,7 +592,7 @@ method MarshallMessage_GetRequest(c:CMessage) returns (val:V)
     ensures  ValInGrammar(val, CMessage_GetRequest_grammar());
     ensures  ValidVal(val);
     ensures  parse_Message_GetRequest(val) == c;
-    ensures  0 <= SizeOfV(val) < MaxPacketSize() - 32;
+    ensures  0 <= SizeOfV(val) < MaxPacketSize() - 0x10_0020;
 {
     val := MarshallKey(c.k_getrequest);
 }
@@ -606,7 +603,7 @@ method MarshallMessage_SetRequest(c:CMessage) returns (val:V)
     ensures  ValInGrammar(val, CMessage_SetRequest_grammar());
     ensures  ValidVal(val);
     ensures  parse_Message_SetRequest(val) == c;
-    ensures  0 <= SizeOfV(val) < MaxPacketSize() - 32;
+    ensures  0 <= SizeOfV(val) < MaxPacketSize() - 0x10_0020;
 {
     var k_setrequest := MarshallKey(c.k_setrequest);
     var v_setrequest := MarshallOptionalValue(c.v_setrequest);
@@ -620,7 +617,7 @@ method MarshallMessage_Reply(c:CMessage) returns (val:V)
     ensures  ValInGrammar(val, CMessage_Reply_grammar());
     ensures  ValidVal(val);
     ensures  parse_Message_Reply(val) == c;
-    ensures  0 <= SizeOfV(val) < MaxPacketSize() - 32;
+    ensures  0 <= SizeOfV(val) < MaxPacketSize() - 0x10_0020;
 {
     var k_reply := MarshallKey(c.k_reply);
     var v := MarshallOptionalValue(c.v);
@@ -634,7 +631,7 @@ method MarshallMessage_Redirect(c:CMessage) returns (val:V)
     ensures  ValInGrammar(val, CMessage_Redirect_grammar());
     ensures  ValidVal(val);
     ensures  parse_Message_Redirect(val) == c;
-    ensures  0 <= SizeOfV(val) < MaxPacketSize() - 32;
+    ensures  0 <= SizeOfV(val) < MaxPacketSize() - 0x10_0020;
 {
     var k_redirect := MarshallKey(c.k_redirect);
     var ep := MarshallEndPoint(c.id);
@@ -648,7 +645,7 @@ method MarshallMessage_Shard(c:CMessage) returns (val:V)
     ensures  ValInGrammar(val, CMessage_Shard_grammar());
     ensures  ValidVal(val);
     ensures  parse_Message_Shard(val) == c;
-    ensures  0 <= SizeOfV(val) < MaxPacketSize() - 32;
+    ensures  0 <= SizeOfV(val) < MaxPacketSize() - 0x10_0020;
 {
     var k_redirect := MarshallKeyRange(c.kr);
     var ep := MarshallEndPoint(c.recipient);
@@ -662,7 +659,7 @@ method MarshallMessage_Delegate(c:CMessage) returns (val:V)
     ensures  ValInGrammar(val, CMessage_Delegate_grammar());
     ensures  ValidVal(val);
     ensures  parse_Message_Delegate(val) == c;
-    ensures  0 <= SizeOfV(val) < MaxPacketSize() - 32;
+    ensures  0 <= SizeOfV(val) < MaxPacketSize() - 0x10_0020;
 {
     var range := MarshallKeyRange(c.range);
     var h := MarshallHashtable(c.h);
@@ -681,7 +678,7 @@ method MarshallMessage_Delegate(c:CMessage) returns (val:V)
             { lemma_mul_is_distributive_add_forall(); } 
         (16 + max_key_len()) + (16 + max_key_len()) + 8 + |c.h| * 8 + |c.h| * max_key_len() + |c.h| * 8 + |c.h| * max_val_len();
         <
-        MaxPacketSize() - 32;
+        MaxPacketSize() - 0x10_0020;
     }
 
 }
@@ -691,7 +688,7 @@ method MarshallMessage(c:CMessage) returns (val:V)
     ensures  ValInGrammar(val, CMessage_grammar());
     ensures  ValidVal(val);
     ensures  parse_Message(val) == c;
-    ensures  0 <= SizeOfV(val) < MaxPacketSize() - 24;
+    ensures  0 <= SizeOfV(val) < MaxPacketSize() - 0x10_0018;
 {
     if c.CGetRequest? {
         var msg := MarshallMessage_GetRequest(c);  
@@ -742,8 +739,6 @@ method MarshallCSingleMessage(c:CSingleMessage) returns (val:V)
 ////////////////////////////////////////////////////////////////////////
 
 function AbstractifyBufferToLSHTPacket(src:EndPoint, dst:EndPoint, data:seq<byte>) : LSHTPacket
-    requires EndPointIsValidPublicKey(src);
-    requires EndPointIsValidPublicKey(dst);
 {
     LPacket(AbstractifyEndPointToNodeIdentity(dst),
            AbstractifyEndPointToNodeIdentity(src),
@@ -782,8 +777,8 @@ function AbstractifyNetPacketToShtPacket(net:NetPacket) : Packet
 
 predicate NetPacketIsAbstractable(net:NetPacket)
 {
-      EndPointIsValidPublicKey(net.src)
-    && EndPointIsValidPublicKey(net.dst)
+      EndPointIsAbstractable(net.src)
+    && EndPointIsAbstractable(net.dst)
 }
 
 predicate NetPacketsIsAbstractable(netps:set<NetPacket>)
